Clarifications in n-step proof

Coq/Payoff/CutPayoffN.v
@@ -1,5 +1,4 @@
-(* Some (unfinished) attempts to generalize proof about cutPayoff
-   to n step contract reduction *)
+(* Lemmas and sketch of the proof of the n-step reduction *)
 Require Import Tactics.
 Require Import ILSyntax.
 Require Import ILSemantics.
@@ -77,40 +76,140 @@ Lemma fromContr_ILsem_RedN_exists c c' n t0 extp envp il_e il_e' disc p1 p2 extI
 Proof.
 Admitted.
 
-Definition cutPayoff_sound c n :=
+Definition cutPayoff_sound c n g n0 :=
   forall envC extC (il_e : ILExpr) (extIL : ExtEnv' ILVal) (envP : EnvP) (extP : ExtEnvP)
-         (v' : ILVal) m n0 p1 p2 curr v trace (disc : nat -> R ) tenv,
+         (v' : R) m p1 p2 curr v trace (disc : nat -> R ) tenv,
   (forall a a', Asset.eqb a a' = true) ->
   (forall l t, fromVal (extC l t) = extIL l t) ->
+  TypeExt extC ->
+  TypeEnv g envC ->
+  g |-C c ->
   IsClosedCT c ->
   fromContr c (ILTexpr (Tnum n0)) = Some il_e ->
   C[|Translate (Tnum n0) c|] envC extC tenv = Some trace ->
-  m + n = horizon c tenv ->
+  n + m = horizon c tenv ->
   sum_list (map (fun t => (disc t * trace t p1 p2 curr)%R)
                 (seq (n+n0) m)) = v ->
-  IL[|cutPayoff il_e|] extIL tenv 0 (n+n0) disc p1 p2 = Some v'->
-  fromVal (RVal v) = v'.
+  IL[|cutPayoff il_e|] extIL tenv 0 (n+n0) disc p1 p2 = Some (ILRVal v')->
+  fromVal (RVal v) = ILRVal v'.
 
 Hint Resolve delay_empty_trace.
 
-Lemma cutPayoff_sound_base c : cutPayoff_sound c 0.
+Lemma cutPayoff_sound_base c g t0 : cutPayoff_sound c 0 g t0.
 Proof.
   unfold cutPayoff_sound. intros.
   eapply Contr_translation_sound with (tenv:=tenv) (envC:=envC) (disc:=disc); eauto;
   try rewrite plus_0_r in *; try rewrite plus_0_l in *; subst; try eassumption; try reflexivity.
-  erewrite ILexpr_eq_cutPayoff_at_n with (c:=c) (t0:=(ILTexpr (Tnum n0))); try eassumption. reflexivity.
-  simpl. apply not_true_is_false. intro. apply Nat.ltb_lt in H4. omega.
+  erewrite ILexpr_eq_cutPayoff_at_n with (c:=c) (t0:=(ILTexpr (Tnum t0))); try eassumption. reflexivity.
+  simpl. apply not_true_is_false. intro. apply Nat.ltb_lt in H7. omega.
 Qed.
 
-Lemma cp_Scale_inversion c n e :
-  cutPayoff_sound (Scale e c) n -> cutPayoff_sound c n.
+Lemma cutPayoff_sound_1 c g n0 : cutPayoff_sound c 1 g n0.
 Proof.
+  induction c; intros until tenv; intros A Xeq TyExt TyEnv TyC Hclosed TC Cs Hor Sum ILs; inversion Hclosed; inversion TyC.
+  - (* zero *)intros. inversion Hor.
+  - (* let *)
+    intros. simpl in *.
+    option_inv_auto.
+  - (* transf *)
+    intros. simpl in *. option_inv_auto. unfold compose in *. some_inv.
+    (*rewrite delay_trace_n_m; try omega. replace (S t0 - t0) with 1 by omega. simpl.
+    unfold empty_trans. replace ((disc _) * 0 + 0)%R with 0%R by ring.*)
+    destruct (Party.eqb p p0).
+    + simpl in *. some_inv. assert (m = 0) by omega. subst. reflexivity.
+    + simpl in *. assert (n0 <? S n0 = true). apply ltb_lt. omega.
+      assert (m = 0) by omega. subst.
+      rewrite H in ILs. some_inv. reflexivity.
+  - (* scale *)
+    intros. simpl in *. option_inv_auto. some_inv. subst. simpl in *. option_inv_auto.
+    destruct_vals. some_inv. subst. rewrite <- delay_scale_trace. unfold scale_trace, compose, scale_trans.
+    rewrite summ_list_common_factor. rewrite <- fromVal_RVal_eq. apply fromVal_RVal_f_eq.
+    erewrite <- cutPayoff_eq_compiled_expr in H7; try eassumption.
+    + eapply Exp_translation_sound with (t0':=0); try (simpl in *; some_inv; subst); try eassumption. simpl.
+      rewrite Zplus_0_r. eassumption.
+    + eapply IHc; eauto. autounfold in *. simpl.
+      rewrite H1. reflexivity.
+  - (* translate *)
+    intros. subst. simpl in *. option_inv_auto.
+    destruct n.
+    + simpl in *. destruct (horizon c tenv) eqn:Hhor.
+      * inversion Hor.
+        (* simpl. eapply IHc; eauto. rewrite adv_ext_0 in H1. rewrite H1. reflexivity. rewrite Hhor. reflexivity. *)
+      * simpl in *. eapply IHc; simpl;eauto. unfold liftM,compose,pure,bind.
+        rewrite adv_ext_0 in H2. rewrite H2. reflexivity.
+        inversion Hor. subst. rewrite delay_trace_0. reflexivity.
+    + simpl in *.
+      eapply Contr_translation_sound with (disc:=disc) (envC:=envC) (tenv:=tenv) (t0':=0);
+        eauto; try reflexivity. simpl.
+      unfold liftM,compose,bind,pure. erewrite adv_ext_iter in H2. rewrite Zpos_P_of_succ_nat in H2. rewrite plus_0_r.
+      rewrite plus_comm. rewrite Zpos_P_of_succ_nat. rewrite Nat2Z.inj_add.
+      replace (Z.succ (Z.of_nat n0 + Z.of_nat n)) with  (Z.of_nat n0 + Z.succ (Z.of_nat n))%Z by ring.
+      rewrite H2. reflexivity. rewrite plus_0_r. simpl.
+      rewrite delay_trace_iter. replace (S n + n0) with (n + S n0) by ring.
+      destruct (horizon c tenv) eqn:Hhor.
+      * inversion Hor.
+      * unfold plus0. simpl in *. inversion Hor. subst.
+        (* replace (S n + S n0 - 1) with (n + (S (S n0) - 1)) by omega. *)
+        rewrite sum_delay. simpl.
+        simpl. replace (n + S n0) with (S (n0 + n)) by ring.
+           replace (S (n0 + n)) with (S (n + n0)) by ring. reflexivity.
+      * erewrite <- ILexpr_eq_cutPayoff_at_n in ILs. eassumption. eauto. eauto. simpl.
+        apply not_true_is_false. unfold not. intros. apply ltb_lt in H. omega.
+  - (* Both *)
+    admit.
+  - (* If *)
+    admit.
 Admitted.
 
-Lemma cp_Translate_inversion c t0 n :
-  cutPayoff_sound (Translate t0 c) n -> cutPayoff_sound c n.
+Lemma cp_Scale_inversion c n e il G t0:
+  G |-E e ∶ REAL ->
+  (fromExp (ILTexprZ (ILTexpr (Tnum t0))) e = Some il) ->
+  cutPayoff_sound (Scale e c) n G t0 -> cutPayoff_sound c n G t0.
 Proof.
+  intros TyE He H. unfold cutPayoff_sound in H.
+  intros until tenv; intros A Xeq TyExt TyEnv TyC Hclosed TC Cs Hor Sum ILs.
+  assert (Hadv : TypeExt (adv_ext (Z.of_nat t0) extC) ) by (apply adv_ext_type;apply TyExt).
+  assert (HH := Esem_typed_total _ _ _ _ _ TyE TyEnv Hadv).
+  destruct HH as [r H']. destruct H' as [Hr Hc]. inversion Hc. subst.
+  simpl in *. option_inv_auto.
+  eapply H with (il_e := (ILBinExpr ILMult il il_e)) (trace:=delay_trace t0 (scale_trace b x));eauto; simpl in *; unfold liftM,liftM2,compose,pure,bind.
+  - rewrite He. rewrite TC. reflexivity.
+  - rewrite H1.
+    rewrite Hr.
+    simpl. reflexivity.
+  - admit.
+  - rewrite ILs. admit.
 Admitted.
+
+Lemma cp_Translate_inversion_0 c n g t0:
+  cutPayoff_sound (Translate (Tnum 0) c) n g t0 -> cutPayoff_sound c n g t0.
+Proof.
+  intros H.
+  intros until tenv; intros A Xeq TyExt TyEnv TyC Hclosed TC Cs Hor Sum ILs.
+  simpl in *. option_inv_auto. unfold cutPayoff_sound in *.
+  eapply H;eauto. simpl. unfold liftM,liftM2,compose,pure,bind.
+  - rewrite adv_ext_iter. replace (Z.of_nat t0 + 0)%Z with (Z.of_nat t0) by omega.
+    rewrite H1. rewrite delay_trace_iter. reflexivity.
+  - simpl. rewrite Hor. destruct (horizon c tenv);reflexivity.
+Qed.
+
+
+Lemma cp_Translate_inversion c n g t0:
+  cutPayoff_sound (Translate (Tnum 1) c) (1+n) g t0 -> cutPayoff_sound c n g (S t0).
+Proof.
+  intros H.
+  intros until tenv; intros A Xeq TyExt TyEnv TyC Hclosed TC Cs Hor Sum ILs.
+  simpl in *. option_inv_auto. unfold cutPayoff_sound in *.
+  eapply H;eauto. simpl. unfold liftM,liftM2,compose,pure,bind.
+  - rewrite adv_ext_iter.
+     assert (Ht0 :(Z.pos (Pos.of_succ_nat t0)) = (Z.of_nat t0 + 1)%Z).
+     {rewrite Zpos_P_of_succ_nat. omega. }
+     rewrite Ht0 in *. rewrite H1. reflexivity.
+  - simpl. rewrite Hor. unfold plus0. destruct (horizon c tenv);try reflexivity. admit.
+  - rewrite delay_trace_iter. replace (n + S t0) with (S n + t0) by omega. reflexivity.
+  - replace (S n + t0) with (n + S t0) by omega. assumption.
+ Admitted.
+
 
 Lemma sum_delay_n':
   forall (n n0 : nat) (tr : Trace) (p1 p2 : Party) (curr : Asset) (f : nat -> R) (t0 n1 : nat),
@@ -119,19 +218,19 @@ Lemma sum_delay_n':
 Proof.
   Admitted.
 
-Lemma cp_sound_translate_1 c n :
-  cutPayoff_sound c n -> cutPayoff_sound (Translate (Tnum 1) c) (1 + n).
+Lemma cp_sound_translate_1 c n g t0:
+  cutPayoff_sound c n g (S t0) -> cutPayoff_sound (Translate (Tnum 1) c) (1 + n) g t0.
 Proof.
   unfold cutPayoff_sound.
-  intros until tenv; intros A Xeq TC CC Cs Hor Sm ILs.
-  inversion TC.
-  eapply H with (m:=m) (n0:= S n0);eauto.
-  + rewrite Equivalence.transl_iter in Cs. replace (S n0) with (n0 + 1) by ring.
+  intros until tenv; intros A Xeq TyExt TyEnv TyC Hclosed TC Cs Hor Sum ILs.
+  inversion Hclosed. inversion TyC. subst.
+  eapply H with (m:=m);eauto.
+  + rewrite Equivalence.transl_iter in Cs. replace (S t0) with (t0 + 1) by ring.
     apply Cs.
   + simpl in *. destruct (horizon c tenv). destruct m;simpl in *;tryfalse.
     simpl in Hor. omega.
-  + simpl in *. replace (n + S n0) with (S (n + n0)) by ring. eapply Sm.
-  + replace (n + S n0) with (S (n + n0)) by ring. eapply ILs.
+  + simpl in *. replace (n + S t0) with (S (n + t0)) by ring. reflexivity.
+  + replace (n + S t0) with (S (n + t0)) by ring. eapply ILs.
 Qed.
 
 Fixpoint transl_one_iter (n : nat) (c : Contr) :=
@@ -143,27 +242,31 @@ Fixpoint transl_one_iter (n : nat) (c : Contr) :=
 (* I think, this property is required for the n-step proof *)
 Lemma cp_summ c n :
   forall envC extC (il_e : ILExpr) (extIL : ExtEnv' ILVal) (envP : EnvP) (extP : ExtEnvP)
-         (v' : ILVal) m n0 p1 p2 curr v v'' trace (disc : nat -> R ) tenv,
+         (v' : R) m n0 p1 p2 curr v v' trace (disc : nat -> R ) tenv,
     (forall a a', Asset.eqb a a' = true) ->
     (forall l t, fromVal (extC l t) = extIL l t) ->
     IsClosedCT c ->
     fromContr c (ILTexpr (Tnum n0)) = Some il_e ->
-    C[|Translate (Tnum n0) c|] envC extC tenv = Some trace ->
+    C[|c|] envC (adv_ext (Z.of_nat n0) extC) tenv = Some trace ->
     m + n = horizon c tenv ->
     sum_list (map (fun t => (disc t * trace t p1 p2 curr)%R)
                   (seq (n+n0) m)) = v ->
-    IL[|cutPayoff il_e|] extIL tenv 0 (n+n0) disc p1 p2 = Some v' ->
-    fromVal (RVal v) = v' ->
-    IL[|cutPayoff il_e|] extIL tenv 0 (1+n+n0) disc p1 p2 = Some (ILRVal v'') ->
-    v' = ILRVal (trace (n+n0)%nat p1 p2 curr + v'')%R.
+    IL[|cutPayoff il_e|] extIL tenv 0 (1+n) disc p1 p2 = Some (ILRVal v') ->
+    IL[|cutPayoff il_e|] extIL tenv 0 n disc p1 p2 =
+    Some (ILRVal (disc n * delay_trace n0 trace n p1 p2 curr + v')%R).
 Proof.
   Admitted.
-  
-Lemma cutPayoff_sound_step c n :
-      cutPayoff_sound c n -> cutPayoff_sound c (1 + n).
+
+Lemma ILRVal_plus v v' l: ILRVal (l + v) = ILRVal (l + v') -> ILRVal v = ILRVal v'.
+Proof.
+  intros H. apply f_equal. inversion H. eapply Rplus_eq_reg_l;eauto.
+Qed.
+
+Lemma cutPayoff_sound_step c n g :
+      cutPayoff_sound c n g 0 -> cutPayoff_sound c (1 + n) g 0.
 Proof.
   generalize dependent n.
-  induction c; intros until tenv; intros A Xeq TC CC Cs Hor S ILs.
+  induction c;intros until tenv; intros A Xeq TyExt TyEnv TyC Hclosed TC Cs Hor Sum ILs; inversion Hclosed; inversion TyC.
   - (* zero *)
     simpl in *. some_inv. subst. simpl in *.
     unfold compose,bind,pure in *. some_inv. rewrite sum_of_map_empty_trace; auto.
@@ -175,51 +278,63 @@ Proof.
     destruct b0.
     + simpl in *. assert (Hmeq0 : m=0) by omega. subst. simpl. some_inv. reflexivity.
     + simpl in *. assert (Hmeq0 : m=0) by omega. assert (Hneq0 : n = 0 ) by omega. subst. simpl.
-      rewrite plus_0_l in *.
-      assert (Hlt_true : (n0 <? S n0) = true). apply Nat.ltb_lt. omega.
-      rewrite Hlt_true in *. some_inv. reflexivity.
+      rewrite plus_0_l in *.  some_inv. reflexivity.
   - (* scale *)
     intros. simpl in *. option_inv_auto. some_inv. subst. simpl in *. option_inv_auto.
     destruct_vals. some_inv. subst. rewrite delay_trace_scale.
     unfold scale_trace, compose, scale_trans.
     rewrite summ_list_common_factor. rewrite <- fromVal_RVal_eq. apply fromVal_RVal_f_eq.
-    + erewrite <- cutPayoff_eq_compiled_expr in H5; try eassumption.
+    + erewrite <- cutPayoff_eq_compiled_expr in H8; try eassumption.
       eapply Exp_translation_sound with (t0':=0) (envT:=tenv) (envC:=envC);
         try (simpl in *; some_inv; subst); try eassumption.
-      rewrite Z.add_0_r. assumption.
-    + inversion TC. apply cp_Scale_inversion in H.
-      eapply IHc with (envC:=envC); eauto. simpl. autounfold.
+    + eapply cp_Scale_inversion in H;eauto.
+      eapply IHc with (envC:=envC); eauto.
+      simpl. autounfold.
       rewrite H2. reflexivity.
   - (* translate *)
     intros.
     simpl in *. option_inv_auto. rewrite delay_trace_swap.
     inversion TC. subst. simpl in *.
-    rename n1 into t0.
     simpl in *.
     rewrite adv_ext_iter in H2.
-    replace (Z.of_nat n0 + Z.of_nat t0)%Z with (Z.of_nat (t0 + n0)) in *.
-    rewrite delay_trace_iter.
-    destruct t0.
-    * apply cp_Translate_inversion in H.
-      rewrite add_0_r. simpl in *. rewrite <- fromVal_RVal_eq.
+    rewrite delay_trace_iter. rewrite add_0_l in *. rewrite add_0_r in *.
+    destruct n0.
+    * simpl in *.
+      apply cp_Translate_inversion_0 in H.
       eapply IHc with (envC:=envC);eauto.
-      simpl. autounfold. rewrite H2. reflexivity.
-      destruct (horizon c tenv);destruct m;simpl in *;tryfalse;auto.
-    * apply cp_Translate_inversion in H.
-      destruct t0. unfold cutPayoff_sound in H.
-      ** eapply H with (m:=m) (n0:= S n0);eauto.
-         *** simpl. autounfold.
-             (* replace (Z.of_nat n0 + 1)%Z with (1 + Z.of_nat n0)%Z by ring. *)
-             (* rewrite succ_of_nat with (t:=0%Z). simpl.          *)
-             simpl in H2. rewrite H2. autounfold. reflexivity.
-         *** simpl in *. destruct (horizon c tenv). destruct m;simpl in *; tryfalse.
-             simpl in *. omega.
-         *** simpl. replace (n0 +1) with (S n0) by ring.
-             replace (n + S n0) with (S (n + n0)) by ring. reflexivity.
-         *** replace (n + S n0) with (S (n + n0)) by ring. assumption.
+      simpl. autounfold. rewrite H2. reflexivity. simpl in *.
+      destruct (horizon c tenv);simpl in *;tryfalse. apply Hor.
+      rewrite add_0_r in *. reflexivity. rewrite add_0_r in *. auto.
+    * unfold cutPayoff_sound in H.
+      remember (sum_list
+       (map (fun t1 : nat => (disc t1 * delay_trace (S n0) x0 t1 p1 p2 curr)%R)
+            (seq (S n) m))) as q.
+      rewrite add_0_r in *.
+      apply ILRVal_plus with (l:= (disc n * delay_trace (S n0) x0 n p1 p2 curr)%R).
+      rewrite <- fromVal_RVal_eq.
+      eapply H with (tenv:=tenv) (disc:=disc) (m:=1+m);eauto.
+      ** simpl. rewrite add_0_r in *. eauto.
+      ** simpl. unfold liftM,liftM2,compose,pure,bind.
+         rewrite Zpos_P_of_succ_nat in *. rewrite <- Nat2Z.inj_succ.
+         rewrite adv_ext_iter.
+         replace (0 + Z.of_nat (S n0))%Z with (Z.of_nat (S n0)) in * by ring.
+         rewrite H2. reflexivity.
+      ** admit.
+      ** rewrite delay_trace_iter. rewrite add_0_r in *.
+         simpl in *. subst q. reflexivity.
+      ** eapply cp_summ with (n0 :=1+n0);eauto.
+         unfold plus0 in *. destruct (horizon c tenv);tryfalse;eauto. admit.
+  - (* Both*)
+    (* We split values on two summands an apply induction hypothes
+       Here we use an inversion principle for [both] (similar to [scale]) to
+       obtain the premises for IHs *)
+    admit.
+  - (* If-within *)
+    (* We proceed by case analisys on the outcome of evaluation of the contition.
+       We perform inner induction on number of iteration for if-within construct *)
 Admitted.
 
-Theorem cutPayoff_sound_n_steps c n: cutPayoff_sound c n.
+Theorem cutPayoff_sound_n_steps c n g : cutPayoff_sound c n g 0.
 Proof.
   induction n.
   - apply cutPayoff_sound_base.
